Add thread-local var spec and fix race condition steps

Examples/TicketLock.v
@@ -1,5 +1,6 @@
 From LHL.Core Require Import
   Program
+  ProgramRules
   Specs
   Logic
   LogicFacts
@@ -11,15 +12,17 @@ From LHL.Examples Require Import
   LockSpec
   FAISpec
   YieldSpec
-  CounterSpec.
+  CounterSpec
+  VarSpec.
 
 From Coq Require Import
   Arith.PeanoNat.
 
-Definition Underlay := FAISig |+| CounterSig |+| YieldSig.
+Definition Underlay := FAISig |+| CounterSig |+| YieldSig |+| VarSig nat.
 
 Definition acq : Prog Underlay unit :=
   my_tick <- call FAI;
+  _ <- call (SetVar my_tick);
   while
     (cur_tick <- call Get; ret (negb (cur_tick =? my_tick)))
     (call Yield).
@@ -35,7 +38,7 @@ Definition ticketLockImpl : Impl Underlay LockSig :=
 
 Definition E := Underlay.
 Definition F := LockSig.
-Definition VE := tensorSpec faiSpec (tensorSpec counterSpec yieldSpec).
+Definition VE := tensorSpec faiSpec (tensorSpec counterSpec (tensorSpec yieldSpec (varSpec nat))).
 Definition VF := lockSpec.
 
 Definition Relt := Relt VE VF.
@@ -62,3 +65,16 @@ Definition Posts (i : ThreadName) {A} (m : LockSig A) : Post A :=
 
 Theorem ticketLockCorrect :
   VerifyImpl VE VF Rely Guar Precs ticketLockImpl Posts.
+split.
+admit.
+split.
+admit.
+split.
+admit.
+intros.
+destruct m.
+simpl.
+unfold acq.
+{
+  
+}
