Examples/CounterSpec.v
@@ -8,14 +8,23 @@ Variant CounterSig : ESig :=
 
 Variant CounterState :=
 | CounterIdle (n : nat)
-| CounterIncRunning (i : ThreadName) (n : nat)
-| CounterGetRunning (i : ThreadName) (n : nat).
+| CounterGetCalled (i : ThreadName) (n : nat)
+| CounterIncCalled (i : ThreadName) (n : nat)
+| CounterUB.
 
 Variant CounterStep : CounterState -> ThreadEvent CounterSig -> CounterState -> Prop :=
-| CounterCallInc i n : CounterStep (CounterIdle n) (i, CallEv Inc) (CounterIncRunning i n)
-| CounterRetInc i n : CounterStep (CounterIncRunning i n) (i, RetEv Inc tt) (CounterIdle (S n))
-| CounterCallGet i n : CounterStep (CounterIdle n) (i, CallEv Get) (CounterGetRunning i n)
-| CounterRetGet i n : CounterStep (CounterGetRunning i n)  (i, RetEv Get n) (CounterIdle n).
+| CounterCallInc i n :
+  CounterStep (CounterIdle n) (i, CallEv Inc) (CounterIncCalled i n)
+| CounterRetInc i n :
+  CounterStep (CounterIncCalled i n) (i, RetEv Inc tt) (CounterIdle (S n))
+| CounterCallGet i n :
+  CounterStep (CounterIdle n) (i, CallEv Get) (CounterGetCalled i n)
+| CounterRetGet i n :
+  CounterStep (CounterGetCalled i n) (i, RetEv Get n) (CounterIdle n)
+| CounterRaceInc i j n :
+  CounterStep (CounterIncCalled i n) (j, CallEv Inc) CounterUB
+| CounterStepUB e :
+  CounterStep CounterUB e CounterUB.
 
 Definition counterSpec : Spec CounterSig := {|
   State := CounterState;
