Examples/VarSpec.v
@@ -1,0 +1,50 @@
+From LHL.Core Require Import
+  Specs
+  Traces
+  Program.
+
+From LHL.Util Require Import
+  Util.
+
+Variant VarSig {S} : ESig :=
+| SetVar : S -> VarSig unit
+| GetVar : VarSig S.
+Arguments VarSig : clear implicits.
+
+Variant VarValue {S} :=
+| VarUnset
+| VarIdle (s : S)
+| VarSetCalled (s : S)
+| VarGetCalled (s : S).
+Arguments VarValue : clear implicits.
+
+Definition VarState S :=
+  ThreadName -> VarValue S.
+
+Variant VarStep {S} : VarState S -> ThreadEvent (VarSig S) -> VarState S -> Prop :=
+| VarCallSet i (m m' : VarState S) s t :
+  m i = VarIdle s ->
+  m' i = VarSetCalled t ->
+  differ_pointwise m m' i ->
+  VarStep m (i, CallEv (SetVar t)) m'
+| VarRetSet i (m m' : VarState S) s :
+  m i = VarSetCalled s ->
+  m' i = VarIdle s ->
+  differ_pointwise m m' i ->
+  VarStep m (i, RetEv (SetVar s) tt) m'
+| VarCallGet i m m' s :
+  m i = VarIdle s ->
+  m' i = VarGetCalled s ->
+  differ_pointwise m m' i ->
+  VarStep m (i, CallEv GetVar) m'
+| VarRetGet i m m' s :
+  m i = VarGetCalled s ->
+  m' i = VarIdle s ->
+  differ_pointwise m m' i ->
+  VarStep m (i, RetEv GetVar s) m'.
+
+Definition varSpec S : Spec (VarSig S) := {|
+  State := VarState S;
+  Step := VarStep;
+  Init := fun _ => VarUnset
+|}.
